Started figuring out how to steal PreCond from old requests via double fupd
The Get() RPC is actually too easy, because we could just change its
spec to say { True } Get() { RET v; (kv [[γ]]↦ some_v -∗ some_v = v) }
and then don't need to ever send the (kv [[γ]]↦ v) over the network.

For Put(), this won't work. For Put(), idempotency holds because a new
Put() will overwrite the old Put(). So, when we run a put, we need to
steal the old Put()'s kv ptsto fact by opening up its request invariant
and taking either its PreCond (if the old Put() never ran) or taking its
PostCond (in case the old Put() already ran). We can only steal the old
requests's (Pre \/ Post) if we know that it'll never be run again; i.e.
we need to update the lastSeqM in order to take the Pre out. This means
that the fupd where we go Pre -> Post now actually also has to invoke
another fupd to even get the Pre.

The the crash obligation is a bit sketchy (it's fupd that gives another
fupd). Knowing that the durable client seqno for Cid is Seq tells us
that as soon as we update the lastSeq on the server to be at least
(Seq - 1), then we can safely steal the old request's (Pre \/ Post).

src/program_proof/lockservice/incr_proof.v
@@ -69,9 +69,79 @@ Definition IncrCrashInvariant (seq:u64) (args:RPCValC) : iProp Σ :=
   "Hfown_oldv" ∷ (("incr_request_" +:+ u64_to_string seq) +:+ "_oldv") f↦ []
 .
 
+Variable γ:kvservice_names.
+
+Context `{!kvserviceG Σ}.
+
+(* This is the double-fupd crash obligation. *)
+Definition KVGetPreClientWeak (cid:u64) (γrpc:durable_rpc_names) (PreCond:iProp Σ): iProp Σ :=
+  ∀ (seq:u64), cid fm[[γrpc.(cseq)]]↦ int.nat seq ={⊤}=∗ (
+            cid fm[[γrpc.(cseq)]]↦ int.nat seq ∗
+                   (own γrpc.(proc) (Excl ()) ∗ cid fm[[γrpc.(lseq)]]≥ int.nat seq) ={⊤}=∗ own γrpc.(proc) (Excl ()) ∗ PreCond
+  ).
+(*
+  Should use up previous γPost to prove this fupd.
+  We want to be able to show
+ *)
+
+Definition IdempotentPre γrpc (cid seq:u64) (PreCond : RPCValC → iProp Σ) : (RPCValC → iProp Σ) :=
+  λ (args:RPCValC),
+        (own γrpc.(proc) (Excl ()) -∗ cid fm[[γrpc.(lseq)]]≥ int.nat seq ={⊤}=∗ own γrpc.(proc) (Excl ()) ∗ PreCond args)%I.
+
+Lemma server_takes_idempotent_request γrpc γPost γPre (cid key va:u64) PreCond PostCond req lastSeqM lastReplyM:
+  (int.Z (map_get lastSeqM req.(Req_CID)).1 < int.Z req.(Req_Seq))%Z →
+  is_durable_RPCServer γrpc -∗
+  is_durable_RPCRequest γrpc γPost γPre (IdempotentPre γrpc req.(Req_CID) req.(Req_Seq) PreCond) (PostCond) req -∗
+  RPCServer_durable_own γrpc lastSeqM lastReplyM ={⊤}=∗
+  PreCond req.(Req_Args) ∗
+  RPCServer_durable_own_processing γrpc req lastSeqM lastReplyM.
+Proof.
+  intros Hrseq.
+  iIntros "HserverInv HreqInv Hsown".
+
+  iInv "HreqInv" as "[#>Hreqeq_lb Hcases]" "HMClose".
+  iNamed "Hsown".
+
+  iDestruct "Hcases" as "[[>Hunproc [>Hbad|Hpre]]|[#>Hlseq_lb _]]".
+  {
+    iDestruct (own_valid_2 with "Hproc_own Hbad") as %H; contradiction.
+  }
+  {
+    iDestruct "Hpre" as "[>HγPre HidemPre]".
+    iSpecialize ("HidemPre" with "[Hproc_own]").
+    {  done. }
+    (* Expectedly stuck trying to show req.cid fm[lseq]≥ req.seq to use the
+       HidemPre fupd Indeed, we won't be able to take PreCond out of the old
+       request until we actually update the seqno on durable storage. Otherwise,
+       we could be holding the proc token, so we know no one else is currently
+       processing the old request, then we steal PreCond from the old request
+       invariant, then we could crash before we update lastSeq, and then after
+       restarting, the old request might *actually* be run again, so it needs
+       its PreCond.
+
+       So, we can only actually get the PreCond as soon as we actually update
+       the lastSeq. This means the core function would not be given [PreCond], but
+       [(own proc ∗ fm[lseq]≥ fact) ={⊤}=∗ PreCond].
+
+       This'll also mean the fupd where we go from PreCond -> PostCond must
+       happen at the same time as the lseq update.
+     *)
+Admitted.
+
+
+Definition IncrServer_core_own (srv:loc) : iProp Σ :=
+  ∃ (kck kvserver:loc),
+  "Hkvserver" ∷ srv ↦[IncrServer.S :: "kvserver"] #kvserver ∗
+  "Hkck" ∷ srv ↦[IncrServer.S :: "kck"] #kck ∗
+  "His_kvserver" ∷ is_kvserver γ kvserver ∗
+  "Hkck_own" ∷ own_kvclerk γ kck kvserver
+  (* This is using the non-crash-safe version of kvserver in kv_proof.v *)
+  .
+
 Lemma increment_core_indepotent (isrv:loc) (seq:u64) (args:RPCValC) :
   {{{
-       IncrCrashInvariant seq args
+       IncrCrashInvariant seq args ∗
+                        IncrServer_core_own isrv
       (* TODO: add ownership of kck so we can make RPCs with it *)
   }}}
     IncrServer__increment_core #isrv #seq (into_val.to_val args) @ 37 ; ⊤
@@ -82,11 +152,11 @@ Lemma increment_core_indepotent (isrv:loc) (seq:u64) (args:RPCValC) :
        IncrCrashInvariant seq args
   }}}.
 Proof.
-  iIntros (Φ Φc) "Hpre Hpost".
+  iIntros (Φ Φc) "[HincrCrashInv Hisown] Hpost".
   wpc_call; first done.
   { iFrame. }
   unfold IncrCrashInvariant.
-  iNamed "Hpre".
+  iNamed "HincrCrashInv".
   iCache with "Hfown_oldv Hpost".
   {
     iDestruct "Hpost" as "[HΦc _]". iModIntro. by iApply "HΦc".
@@ -134,6 +204,12 @@ Proof.
 
   (* case that no durable oldv chosen *)
   wpc_pures.
+  iNamed "Hisown".
+
+  wpc_bind (struct.loadF _ _ _).
+  wpc_frame.
+  wp_loadField.
+  iNamed 1.
 
   (* Use has_encoding data [] ∨ ... in invariant *)
 
